src/program_proof/barebones_proof.v
@@ -1,0 +1,605 @@
+From Perennial.goose_lang.lib Require Import encoding.
+From Perennial.program_proof Require Import proof_prelude.
+From Perennial.goose_lang Require Import ffi.disk_prelude.
+From Perennial.algebra Require Import deletable_heap.
+From Goose.github_com.mit_pdos.goose_nfsd Require Import barebones common super inode.
+From Perennial.program_proof Require Import disk_lib.
+From Perennial.program_proof Require Import buftxn.specs buf.defs buf.specs txn.specs addr.specs marshal_proof.
+
+Section heap.
+Context `{!heapG Σ}.
+Context `{!crashG Σ}.
+Context `{!lockG Σ}.
+Context `{!buftxnG Σ}.
+Implicit Types (v:val).
+Implicit Types (stk:stuckness) (E: coPset).
+
+(* Definition common_NBITBLOCK := disk.block_bytes / 8.
+Definition common_META := 8.
+Definition common_HDRADDRS :=
+Definition common_LOGSIZE := common_HDRADDRS + 2.
+Definition nBlockBitmap diskSz := (diskSz / common_NBITBLOCK) + 1.
+Definition nLog := common_LOGSIZE.
+Definition bnum_BitmapBlockStart := nLog.
+Definition bnum_BitmapInodeStart := bnum_BitmapBlockStart +  *)
+
+Definition common_INODESZ : nat := 128.
+Definition common_INODEBLK : nat := common_INODESZ / disk.block_bytes.
+Definition common_ROOTINUM : nat := 1.
+
+Definition nfstypes__NFS3_OK : nat := 0.
+
+Definition inode_NENTRIES : nat := 8.
+
+Record SuperData : Set := mkSuperData {
+(*   superd_size : nat;
+  superd_nLog : nat;
+  superd_nBlockBitmap : nat;
+  superd_nInodeBitmap : nat;
+  superd_nInodeBlk : nat;
+  superd_maxAddr : nat; *)
+  superd_inodeStartPrecomp : nat;
+}.
+
+Definition is_super super superd : iProp Σ :=
+(*   super ↦[FsSuper.S :: "Size"] #(superd.(superd_size)) ∗
+  super ↦[FsSuper.S :: "nLog"] #(superd.(superd_nLog)) ∗
+  super ↦[FsSuper.S :: "NBlockBitmap"] #(superd.(superd_nBlockBitmap)) ∗
+  super ↦[FsSuper.S :: "NInodeBitmap"] #(superd.(superd_nInodeBitmap)) ∗
+  super ↦[FsSuper.S :: "nInodeBlk"] #(superd.(superd_nInodeBlk)) ∗
+  super ↦[FsSuper.S :: "Maxaddr"] #(superd.(superd_maxAddr)). *)
+  super ↦[FsSuper.S :: "InodeStartPrecomp"] #(superd.(superd_inodeStartPrecomp)) ∗
+  ⌜ superd.(superd_inodeStartPrecomp) = O ⌝. (* this is blatantly false but it doesn't matter that much *)
+
+Record FhData : Set := mkFhData {
+  fhd_ino : nat;
+  fhd_gen : nat;
+}.
+
+Definition fhd2val fhd : val := (#fhd.(fhd_ino), (#fhd.(fhd_gen), #())).
+
+Definition is_fh fhl fhd : iProp Σ :=
+  fhl ↦[Fh.S :: "Ino"] #(fhd.(fhd_ino)) ∗
+  fhl ↦[Fh.S :: "Gen"] #(fhd.(fhd_gen)).
+
+Record InodeEntry : Set := mkInodeEntry {
+  inodee_inum : nat;
+  inodee_name : Ascii.ascii; (* all our names are one character long *)
+}.
+
+Record InodeData : Set := mkInodeData {
+  inoded_inum : nat;
+  inoded_gen : nat;
+  inoded_parent : nat;
+  inoded_entries : vec InodeEntry inode_NENTRIES;
+}.
+
+Definition inoded_children inoded := vmap inodee_inum (inoded_entries inoded).
+Definition inoded_names inoded := vmap inodee_name (inoded_entries inoded).
+
+Definition inoded2fhd inoded := {|
+  fhd_ino := inoded.(inoded_inum);
+  fhd_gen := inoded.(inoded_gen);
+|}.
+
+Definition nat2val (n: nat) := #(n).
+Definition inoded_children_val inoded :=
+  nat2val <$> vec_to_list (inoded_children inoded).
+Definition ascii2val (a: Ascii.ascii) := #(Ascii.nat_of_ascii a).
+Definition inoded_names_val inoded :=
+  ascii2val <$> vec_to_list (inoded_names inoded).
+
+Definition is_inode inodel inoded : iProp Σ :=
+  ∃ sl_contents sl_names,
+  inodel ↦[Inode.S :: "Inum"] #(inoded.(inoded_inum)) ∗
+  inodel ↦[Inode.S :: "Gen"] #(inoded.(inoded_gen)) ∗
+  inodel ↦[Inode.S :: "Parent"] #(inoded.(inoded_parent)) ∗
+  inodel ↦[Inode.S :: "Contents"] (slice_val sl_contents) ∗
+  inodel ↦[Inode.S :: "Names"] (slice_val sl_names) ∗
+  is_slice_small sl_contents uint64T 1 (inoded_children_val inoded) ∗
+  is_slice_small sl_names u8T 1 (inoded_names_val inoded).
+
+(* Definition superd_BitmapBlockStart superd := superd.(superd_nLog).
+Definition superd_BitmapInodeStart superd :=
+  superd_BitmapBlockStart superd + superd.(superd_nBlockBitmap).
+Definition superd_InodeStart superd :=
+  superd_BitmapInodeStart superd + superd.(superd_nInodeBitmap).
+Definition superd_DataStart superd :=
+  superd_InodeStart superd + superd.(superd_nInodeBlk). *)
+(* ... *)
+Definition superd_InodeStart superd :=
+  superd.(superd_inodeStartPrecomp).
+
+(* Definition inum2addr superd inum := {|
+  addrBlock := superd_InodeStart superd + (inum / common_INODEBLK);
+  addrOff := (inum `mod` common_INODEBLK) * common_INODESZ * 8;
+|}. *)
+
+(* simplified inum2addr *)
+Definition inum2addr superd inum := {|
+  addrBlock := superd_InodeStart superd + inum;
+  addrOff := 0;
+|}.
+
+Definition EncNat n := EncUInt64 (U64 (Z.of_nat n)).
+
+Definition encodes_inode i inoded : iProp Σ :=
+  ∃ extra names_bytes,
+  ⌜
+    inode_to_vals i = b2val <$> marshal_proof.encode (
+      [
+        EncUInt64 inoded.(inoded_gen);
+        EncUInt64 inoded.(inoded_parent)
+      ]
+      ++ (EncNat <$> (vec_to_list (inoded_children inoded)))
+      ++ [EncBytes names_bytes]
+    ) ++ extra
+    ∧ u8_to_ascii <$> names_bytes = vec_to_list (inoded_names inoded)
+  ⌝.
+
+Definition buf_encodes_inode {K} (buf: bufDataT K) inoded : iProp Σ :=
+  match buf with
+  | bufInode i => encodes_inode i inoded
+  | _ => False
+  end.
+
+Definition mapsto_txn_inode superd γUnified inoded : iProp Σ :=
+  ∃ i,
+  (|==> mapsto_txn γUnified (inum2addr superd inoded.(inoded_inum)) (bufInode i)) ∗
+  encodes_inode i inoded.
+
+Definition mapsto_inode superd γT inoded : iProp Σ :=
+  ∃ (v: {K & bufDataT K}),
+  buf_encodes_inode (projT2 v) inoded ∗
+  (|==> mapsto (hG := γT) (inum2addr superd inoded.(inoded_inum)) 1 v).
+
+Theorem mapsto_inode_lift inoded superd buftx γT γUnified :
+  (
+    (|==> is_buftxn buftx γT γUnified) ∗
+    mapsto_txn_inode superd γUnified inoded
+  )
+    ==∗
+  (
+    (|==> is_buftxn buftx γT γUnified) ∗
+    mapsto_inode superd γT inoded
+  ).
+Proof.
+  iIntros "[Hbuftxn Hmapsto]".
+  iDestruct "Hmapsto" as (i) "[Hmapsto Hencodes]".
+  iPoseProof (BufTxn_lift_one _ _ _ _ (existT _ _) with "[> Hbuftxn Hmapsto]") as "Hmapsto".
+  {
+    iDestruct "Hbuftxn" as "> Hbuftxn".
+    iDestruct "Hmapsto" as "> Hmapsto".
+    iFrame.
+    eauto.
+  }
+  iDestruct "Hmapsto" as "> [Hbuftxn Hmapsto]".
+  iModIntro.
+  iFrame.
+  iSplitR.
+  1: eauto.
+  iExists _.
+  iFrame.
+  eauto.
+Qed.
+
+Definition mapsto_txn_free_inode superd γUnified inum : iProp Σ :=
+  ∃ i,
+  mapsto_txn γUnified (inum2addr superd inum) (bufInode i).
+
+Definition mapsto_txn_root_inode superd γUnified root_inoded : iProp Σ :=
+  ⌜ root_inoded.(inoded_inum) = common_ROOTINUM ⌝ ∗
+  mapsto_txn_inode superd γUnified root_inoded.
+
+Definition inodee_nonnull inodee := inodee.(inodee_inum) ≠ O.
+
+Definition is_barebones_nfs_super nfsl superd : iProp Σ :=
+  ∃ (superl: loc),
+  nfsl ↦[BarebonesNfs.S :: "fs"] #superl ∗
+  is_super superl superd.
+
+Definition is_barebones_nfs_txn nfsl γUnified : iProp Σ :=
+  ∃ (txnl: loc),
+  nfsl ↦[BarebonesNfs.S :: "txn"] #txnl ∗
+  is_txn txnl γUnified.
+  
+Definition is_barebones_nfs_meta nfsl superd γUnified root_inoded : iProp Σ :=
+  is_barebones_nfs_txn nfsl γUnified ∗
+  is_barebones_nfs_super nfsl superd ∗
+  mapsto_txn_root_inode superd γUnified root_inoded.
+
+Definition is_inode_entry entry name inum :=
+  name = Ascii.nat_of_ascii entry.(inodee_name) ∧
+  inum = entry.(inodee_inum).
+
+Definition non_null_entries_of inoded :=
+  filter inodee_nonnull (vec_to_list inoded.(inoded_entries)).
+
+Definition mapsto_txn_inode_entry superd γUnified entry name inoded : iProp Σ :=
+  ⌜is_inode_entry entry name inoded.(inoded_inum)⌝
+  ∗ mapsto_txn_inode superd γUnified inoded.
+
+Definition mapsto_txn_children root_inoded (name_to_inoded_map : gmap nat InodeData) superd γUnified : iProp Σ :=
+  ([∗ maplist] name ↦ inoded; entry ∈ name_to_inoded_map; (non_null_entries_of root_inoded),
+    mapsto_txn_inode_entry superd γUnified entry name inoded)%I.
+
+Theorem mapsto_txn_children_delete : ∀ root_inoded (name_to_inoded_map: gmap nat InodeData) non_null_set excluded_name superd γUnified inoded,
+  ⌜non_null_entries_of root_inoded ≡ₚ map snd (map_to_list non_null_set)⌝
+  ∗ ⌜name_to_inoded_map !! excluded_name = Some inoded⌝
+  ∗ ([∗ map] name ↦ inoded; entry ∈ name_to_inoded_map; non_null_set,
+    mapsto_txn_inode_entry superd γUnified entry name inoded
+  )
+  -∗
+  ∃ entry,
+    ⌜non_null_set !! excluded_name = Some entry⌝
+    ∗ mapsto_txn_inode_entry superd γUnified entry excluded_name inoded
+    ∗ ([∗ map] name ↦ inoded; entry ∈
+        (delete excluded_name name_to_inoded_map);
+        (delete excluded_name non_null_set), 
+      mapsto_txn_inode_entry superd γUnified entry name inoded
+    ).
+Proof.
+  iIntros (root_inoded name_to_inoded_map non_null_set excluded_name superd γUnified inoded)
+    "(%Hnon_null_set & %Hin_map & Hmapsto)".
+  iDestruct (big_sepM2_lookup_1_some with "Hmapsto") as %[v Hmk].
+  1: eauto.
+  rewrite big_sepM2_delete.
+  2-3: eassumption.
+  iDestruct "Hmapsto" as "[[%Hentry Hinode] Hmapsto]".
+  iFrame.
+  iExists v.
+  eauto.
+Qed.
+
+Theorem mapsto_txn_children_undelete : ∀ root_inoded (name_to_inoded_map: gmap nat InodeData) non_null_set excluded_name superd γUnified inoded entry,
+  ⌜non_null_entries_of root_inoded ≡ₚ map snd (map_to_list non_null_set)⌝
+  ∗ ⌜name_to_inoded_map !! excluded_name = Some inoded⌝
+  ∗ ⌜non_null_set !! excluded_name = Some entry⌝
+  ∗ mapsto_txn_inode_entry superd γUnified entry excluded_name inoded
+  ∗ ([∗ map] name ↦ inoded; entry ∈
+      (delete excluded_name name_to_inoded_map);
+      (delete excluded_name non_null_set), 
+    mapsto_txn_inode_entry superd γUnified entry name inoded
+  )
+  -∗ ([∗ map] name ↦ inoded; entry ∈ name_to_inoded_map; non_null_set,
+    mapsto_txn_inode_entry superd γUnified entry name inoded
+  ).
+Proof.
+  iIntros (root_inoded name_to_inoded_map non_null_set excluded_name superd γUnified inoded entry)
+    "(%Hnon_null_set & %Hin_map & %Hin_set & Hexcluded & Hmapsto)".
+  replace name_to_inoded_map with
+    (<[excluded_name:=inoded]>(delete excluded_name name_to_inoded_map)) at 2.
+  2: {
+    rewrite insert_delete.
+    apply insert_id.
+    assumption.
+  }
+  replace non_null_set with
+    (<[excluded_name:=entry]>(delete excluded_name non_null_set)) at 2.
+  2: {
+    rewrite insert_delete.
+    apply insert_id.
+    assumption.
+  }
+  rewrite big_sepM2_insert.
+  2-3: apply lookup_delete.
+  iFrame.
+Qed.
+
+Definition mapsto_txn_free_inodes used_inums superd γUnified : iProp Σ :=
+  ∀ (free_inum: nat), ⌜In free_inum used_inums⌝ -∗ 
+    mapsto_txn_free_inode superd γUnified free_inum.
+
+Definition used_inums (name_to_inoded_map: gmap nat InodeData) :=
+  common_ROOTINUM :: (map (inoded_inum ∘ snd) (map_to_list name_to_inoded_map)).
+
+Definition is_barebones_nfs (nfsl: loc) root_inoded (name_to_inoded_map: gmap nat InodeData) : iProp Σ :=
+  ∃ superd γUnified,
+  is_barebones_nfs_meta nfsl superd γUnified root_inoded ∗
+  mapsto_txn_children root_inoded name_to_inoded_map superd γUnified ∗
+  mapsto_txn_free_inodes (used_inums name_to_inoded_map) superd γUnified.
+
+Theorem wp_FsSuper__InodeStart superl superd:
+  {{{ is_super superl superd }}}
+    FsSuper__InodeStart #superl
+  {{{ RET #(superd.(superd_inodeStartPrecomp)); is_super superl superd }}}.
+Proof.
+  iIntros (Φ) "(Hsuper & Hsuper_lim) HΦ".
+  wp_call.
+  wp_loadField.
+  iApply "HΦ".
+  iFrame.
+Qed.
+
+Theorem wp_FsSuper__Inum2Addr superl superd inum:
+  {{{ is_super superl superd }}}
+    FsSuper__Inum2Addr #superl #inum
+  {{{ RET (addr2val (inum2addr superd inum)); is_super superl superd }}}.
+Proof.
+  iIntros (Φ) "Hsuper HΦ".
+  wp_call.
+  wp_apply (wp_FsSuper__InodeStart with "Hsuper").
+  rewrite /addr2val.
+  iIntros "Hsuper".
+  wp_pures.
+  wp_call.
+  rewrite /inum2addr.
+  simpl.
+  replace
+    (@word.add _ _ superd.(superd_inodeStartPrecomp) inum)
+    with
+    (U64 (superd.(superd_inodeStartPrecomp) + inum)).
+  2: {
+    rewrite /superd_InodeStart.
+    word_cleanup.
+    unfold word.wrap.
+    rewrite -> Zplus_mod_idemp_r.
+    rewrite -> Zplus_mod_idemp_l.
+    reflexivity.
+  }
+  iApply "HΦ".
+  iFrame.
+Qed.
+
+Theorem wp_Inode__decode bufl (inum: u64) inodel a b inoded:
+  {{{ is_buf bufl a b
+    ∗ buf_encodes_inode b.(bufData) inoded }}}
+    inode.Decode #bufl #inum
+  {{{ RET #inodel;
+    is_buf bufl a b
+    ∗ buf_encodes_inode b.(bufData) inoded
+    ∗ is_inode inodel inoded }}}.
+Proof.
+  iIntros (Φ) "(Hbufl & Hbuf) HΦ".
+  wp_call.
+  wp_apply wp_allocStruct.
+  1: repeat (try constructor; try rewrite zero_slice_val; eauto).
+  iIntros (inodel') "Hinodel".
+  wp_pures.
+  iDestruct "Hbufl" as (data sz) "(Haddr & Hsz & Hdata & Hdirty & Hbuf_addr & Hbuf_sz & Hbuf_nonnull & Hbuf_data)".
+  wp_loadField.
+  rewrite /buf_encodes_inode.
+  destruct b.(bufData); eauto.
+  rewrite /is_buf_data.
+  iDestruct "Hbuf" as (extra names_bytes) "%Hbuf_inode".
+  destruct Hbuf_inode as (Hbuf_children & Hbuf_names).
+  wp_apply (wp_NewDec with "[Hbuf_data]").
+  {
+    replace u8T with byteT by eauto.
+    rewrite -> Hbuf_children.
+    iFrame.
+  }
+  iIntros (dec) "[Hdec %Hdec_data]".
+  wp_pures.
+  iDestruct (struct_fields_split with "Hinodel") as
+    "(Hinodel_inum & Hinodel_gen & Hinodel_parent & Hinodel_contents & Hinodel_names & _)".
+  wp_storeField.
+  wp_apply (wp_Dec__GetInt with "Hdec").
+  iIntros "Hdec".
+  wp_storeField.
+  wp_apply (wp_Dec__GetInt with "Hdec").
+  iIntros "Hdec".
+  wp_storeField.
+  wp_apply (wp_Dec__GetInts with "[Hdec]").
+  {
+    replace (EncNat <$> _) with
+      (EncUInt64 ∘ (U64 ∘ Z.of_nat) <$> vec_to_list (inoded_children inoded)).
+    2: {
+      eapply map_fmap_ext.
+      eauto.
+    }
+    replace (EncUInt64 ∘ (U64 ∘ Z.of_nat) <$> _) with
+      (EncUInt64 <$> (U64 ∘ Z.of_nat <$> vec_to_list (inoded_children inoded))).
+    2: {
+      symmetry.
+      eapply map_fmap_compose.
+    }
+    iFrame.
+    iPureIntro.
+    word_cleanup.
+    rewrite fmap_length vec_to_list_length.
+    eauto.
+  }
+  iIntros (sl_children) "[Hdec Hsl_children]".
+  wp_bind (struct.storeF _ _ _ _).
+  iApply (wp_storeField with "Hinodel_contents").
+  {
+    rewrite /field_ty.
+    simpl.
+    eauto.
+  }
+  iIntros "!> Hinodel_contents".
+  wp_pures.
+  admit. (* no wp_Dec__GetBytes? *)
+Admitted.
+
+Theorem wp_BarebonesNfs__getInode nfsl buftx superd γT γUnified inoded:
+  {{{ is_barebones_nfs_super nfsl superd
+    ∗  (|==> is_buftxn buftx γT γUnified)
+    ∗ mapsto_inode superd γT inoded }}}
+    BarebonesNfs__getInode #nfsl #buftx #(inoded.(inoded_inum))
+  {{{ inodel, RET #inodel;
+    is_barebones_nfs_super nfsl superd
+    ∗ is_inode inodel inoded
+    ∗ (|==> is_buftxn buftx γT γUnified)
+    ∗ mapsto_inode superd γT inoded }}}.
+Proof.
+  iIntros (Φ) "(Hsuper & Hbuftxn & Hinode) HΦ".
+  wp_call.
+  iDestruct "Hsuper" as (superl) "[Hsuperl Hsuper]".
+  wp_loadField.
+  wp_apply (wp_FsSuper__Inum2Addr with "Hsuper").
+  iIntros "Hsuper".
+  wp_pures.
+  rewrite /mapsto_inode.
+  iDestruct "Hinode" as (v) "[Hencodes Hinode]".
+  replace (@word.mul _ _ 128 8) with (U64 (Z.of_nat (128 * 8))) by eauto.
+  destruct v eqn:Hv.
+  simpl.
+  destruct b eqn:Hb; eauto.
+  wp_apply (wp_BufTxn__ReadBuf with "[> Hbuftxn Hinode]").
+  {
+    iDestruct "Hbuftxn" as "> Hbuftxn".
+    iDestruct "Hinode" as "> Hinode".
+    iFrame.
+    iPureIntro.
+    eauto.
+  }
+  iIntros (bufl dirty) "[Hbuf Hbuftxn]".
+  wp_pures.
+  wp_apply (wp_Inode__decode with "[Hencodes Hbuf]").
+  { iFrame. }
+  iIntros "(Hbuf & Hencodes & Hinode)".
+  iApply "HΦ".
+  iDestruct ("Hbuftxn" $! b dirty) as "Hbuftxn".
+  iSplitL "Hsuperl Hsuper".
+  {
+    iExists superl.
+    iFrame.
+  }
+  iSplitL "Hinode".
+  1: iFrame.
+  rewrite Hb.
+  iSpecialize ("Hbuftxn" with "[Hbuf]"). 1: eauto.
+  rewrite sep_exist_l.
+  iExists _.
+  iFrame.
+  (* iDestruct "Hbuftxn" as "> [Hinode Hbuftxn]".
+  iFrame. *)
+  admit. (* fancy update *)
+Admitted.
+
+Theorem wp_BarebonesNfs__getInodeByFh nfsl buftx γT γUnified superd inoded:
+  {{{ (|==> is_buftxn buftx γT γUnified)
+    ∗ is_barebones_nfs_super nfsl superd
+    ∗ mapsto_inode superd γT inoded }}}
+    BarebonesNfs__getInodeByFh #nfsl #buftx (fhd2val (inoded2fhd inoded))
+  {{{ inodel, RET (#inodel, #(U32 nfstypes__NFS3_OK));
+    (|==> is_buftxn buftx γT γUnified)
+    ∗ is_barebones_nfs_super nfsl superd
+    ∗ mapsto_inode superd γT inoded
+    ∗ is_inode inodel inoded }}}.
+Proof.
+  iIntros (Φ) "(Hbuftxn & Hsuper & Hinode) HΦ".
+  wp_call.
+  wp_apply (wp_BarebonesNfs__getInode with "[Hbuftxn Hsuper Hinode]").
+  {
+    iFrame.
+  }
+  iIntros (inodel) "(Hsuper & Hinodel & Hbuftxn & Hinode)".
+  wp_pures.
+  wp_if_destruct.
+  {
+    wp_pures.
+    admit. (* pointer guaranteed non-null *)
+  }
+  iDestruct "Hinodel" as (sl_contents sl_names) "(Hinum & Hgen & Hinode_rest)".
+  wp_loadField.
+  rewrite /inoded2fhd /fhd2val.
+  wp_pures.
+  wp_if_destruct.
+  {
+    rewrite -> base.negb_true in Heqb0.
+    apply bool_decide_eq_false in Heqb0.
+    intuition.
+  }
+  wp_pures.
+  iApply "HΦ".
+  iFrame.
+  iExists sl_contents, sl_names.
+  iFrame.
+Admitted.
+
+Theorem wp_BarebonesNfs__opGetAttr nfsl fhd root_inoded name_to_inoded_map inoded:
+  {{{ is_barebones_nfs nfsl root_inoded name_to_inoded_map
+    ∗ ⌜
+      inoded2fhd inoded = fhd ∧
+      (
+        inoded.(inoded_inum) = common_ROOTINUM
+        ∨ (∃ name, name_to_inoded_map !! name = Some inoded)
+      )
+    ⌝ }}}
+    BarebonesNfs__OpGetAttr #nfsl (fhd2val fhd)
+  {{{ inodel, RET (#inodel, #(U32 nfstypes__NFS3_OK));
+    is_barebones_nfs nfsl root_inoded name_to_inoded_map
+    ∗ is_inode inodel inoded }}}.
+Proof.
+  iIntros (Φ) "(Hbarebones & %Hfd) HΦ".
+  wp_call.
+  iDestruct "Hbarebones" as (superd γUnified)
+    "((Htxn & Hsuper & Hinode_r) & Hinode_c & Hinode_f)".
+  iDestruct "Htxn" as (txnl) "[Htxnl Htxn]".
+  wp_loadField.
+  iPoseProof (is_txn_dup with "Htxn") as "[Htxn Htxn_now]".
+  wp_apply (wp_buftxn_Begin with "Htxn_now").
+  iIntros (buftx γT) "Hbuftxn".
+  wp_pures.
+  destruct Hfd as [Hfd [ Hinum | (name & Hinoded) ]].
+  1: admit. (* root inode *)
+
+  iDestruct "Hinode_c" as (non_null_set) "[%Hnon_null_set Hinode_c]".
+  iPoseProof (mapsto_txn_children_delete with "[Hinode_c]") as (entry) "(%Hin_set & [%Hentry Hinode] & Hinode_c)".
+  1: eauto.
+  subst fhd.
+
+  wp_apply (wp_BarebonesNfs__getInodeByFh with "[Hbuftxn Hsuper Hinode]").
+  {
+    iPoseProof (mapsto_inode_lift with "[Hbuftxn Hinode]") as "Hinode".
+    {
+      iFrame.
+      eauto.
+    }
+    iFrame.
+    admit. (* fancy update *)
+  }
+  iIntros (inodel) "(Hbuftxn & Hsuper & Hinode & Hinodel)".
+  wp_pures.
+  iDestruct "Hinode" as (v) "[Hinode_buf Hinode]".
+  wp_apply (wp_BufTxn__CommitWait _ _ _
+    (<[_:=_]>∅
+  ) with
+    "[Hbuftxn Hinode]").
+  {
+    iFrame.
+    rewrite -> big_sepM_insert by eauto.
+    eauto.
+    admit. (* fancy update *)
+  }
+  iIntros (ok) "Hinode".
+  wp_pures.
+  iApply "HΦ".
+  iFrame.
+  iExists superd, γUnified.
+  iFrame.
+  iSplitL "Htxnl Htxn".
+  {
+    iExists _.
+    iFrame.
+  }
+  iExists non_null_set.
+  iSplit.
+  1: eauto.
+  iApply mapsto_txn_children_undelete.
+  rewrite big_sepM_insert.
+  2: eauto.
+  iDestruct "Hinode" as "[Hinode _]".
+  iFrame.
+  iSplit. 1: eauto.
+  iSplit. 1: eauto.
+  iSplit. 1: eauto.
+  rewrite /mapsto_txn_inode_entry.
+  iSplit. 1: eauto.
+  instantiate (1 := v).
+  destruct v eqn:Hv.
+  rewrite /buf_encodes_inode.
+  destruct b eqn:Hb.
+  1,3: eauto.
+  iExists i.
+  simpl.
+  iFrame.
+  eauto.
+  Unshelve.
+  1-2: eauto.
+Admitted.
+
+End heap.
